ulib/FStar.TwoLevelHeap.fst
@@ -42,13 +42,13 @@ let ref_as_rref #a i r = r
 
 val lemma_as_ref_inj: #a:Type -> #i:rid -> r:rref i a
     -> Lemma (requires (True))
-             (ensures ((ref_as_rref i (as_ref r) = r)))
+             (ensures ((ref_as_rref i (as_ref r) == r)))
        [SMTPat (as_ref r)]
 let lemma_as_ref_inj #a #i r = ()
 
 assume val new_region: unit -> ST rid
       (requires (fun m -> True))
-      (ensures (fun (m0:t) (id:rid) (m1:t) -> exists (h:heap). not(Map.contains m0 id) /\ m1=Map.upd m0 id h))
+      (ensures (fun (m0:t) (id:rid) (m1:t) -> exists (h:heap). not(Map.contains m0 id) /\ m1==Map.upd m0 id h))
 
 let sel (#a:Type) (#i:rid) (m:t) (r:rref i a) = Heap.sel (Map.sel m i) (as_ref r)
 let upd (#a:Type) (#i:rid) (m:t) (r:rref i a) (v:a) = Map.upd m i (Heap.upd (Map.sel m i) (as_ref r) v)
@@ -58,22 +58,22 @@ assume val ralloc: #a:Type -> i:rid -> init:a -> ST (rref i a)
     (ensures (fun m0 x m1 ->
                     let region_i = Map.sel m0 i in
                     (not (Heap.contains region_i (as_ref x))
-                    /\ m1=Map.upd m0 i (Heap.upd region_i (as_ref x) init))))
+                    /\ m1==Map.upd m0 i (Heap.upd region_i (as_ref x) init))))
 
 assume val op_Colon_Equals: #a:Type -> #i:rid -> r:rref i a -> v:a -> ST unit
   (requires (fun m -> True))
-  (ensures (fun m0 _u m1 -> m1= Map.upd m0 i (Heap.upd (Map.sel m0 i) (as_ref r) v)))
+  (ensures (fun m0 _u m1 -> m1== Map.upd m0 i (Heap.upd (Map.sel m0 i) (as_ref r) v)))
 
 assume val op_Bang:#a:Type -> #i:rid -> r:rref i a -> ST a
   (requires (fun m -> True))
-  (ensures (fun m0 x m1 -> m1=m0 /\ x=Heap.sel (Map.sel m0 i) (as_ref r)))
+  (ensures (fun m0 x m1 -> m1==m0 /\ x==Heap.sel (Map.sel m0 i) (as_ref r)))
 
 assume val get: unit -> ST t
   (requires (fun m -> True))
-  (ensures (fun m0 x m1 -> m0=x /\ m1=m0))
+  (ensures (fun m0 x m1 -> m0==x /\ m1==m0))
 
-let modifies (s:Set.set rid) (m0:t) (m1:t) =
-    Map.equal m1 (Map.concat m1 (Map.restrict (Set.complement s) m0))
+let modifies (s:BSet.set rid) (m0:t) (m1:t) =
+    Map.equal m1 (Map.concat m1 (Map.restrict (BSet.complement s) m0))
 
 let fresh_region (i:rid) (m0:t) (m1:t) =
   not (Map.contains m0 i)
