examples/unit-tests/universes/testTwoLevelHeap.fst
@@ -4,7 +4,7 @@ open FStar.TwoLevelHeap
 val test0: #r:rid -> i:int -> v:rref r int -> ST int
   (requires (fun m0 -> Map.contains m0 r))
   (ensures (fun m0 k m1 -> k=i+sel m0 v
-                        /\ modifies Set.empty m0 m1))
+                        /\ modifies BSet.empty m0 m1))
 let test0 #r i v =
   let r = new_region () in
   let x = ralloc r i in
