examples/unit-tests/universes/testheap.fst
@@ -4,7 +4,7 @@ open FStar.Heap
 assume val x : ref int
 assume val y : ref int
 assume val h : heap
-assume DistinctXY: x <> y
+assume DistinctXY: x =!= y
 
 let test0 _ = assert (sel (upd h x 0) x = 0)
 let test1 _ = assert (sel (upd (upd h x 0) y 1) x = 0)
